coq/TypSubst.v
@@ -1,0 +1,171 @@
+Require Import LibTactics.
+Require Import Coq.micromega.Lia.
+Require Import LN_Lemmas.
+Require Export Dispatch.
+
+(* (* B.15 (1) *) *)
+(* Lemma applyty_andl_sub_1 : forall (A1 A2 B B1 B2 : typ) (V:Fty), *)
+(*     TypeWF nil (A1&A2) -> isValFty V -> *)
+(*     ApplyTy (A1&A2) V B -> ApplyTy A1 V B1 -> ApplyTy A2 V B2 -> B1&B2 <: B. *)
+
+(* (* B.15 (2) *) *)
+(* Lemma applyty_andl_sub_2 : forall (A1 A2 B B1 : typ) (V:Fty), *)
+(*     TypeWF nil (A1&A2) -> isValFty V -> *)
+(*     ApplyTy (A1&A2) V B -> ApplyTy A1 V B1 -> NApplyTy A2 V -> B1 <: B. *)
+
+(* (* B.15 (3) *) *)
+(* Lemma applyty_andl_sub_3 : forall (A1 A2 B B2 : typ) (V:Fty), *)
+(*     TypeWF nil (A1&A2) -> isValFty V -> *)
+(*     ApplyTy (A1&A2) V B -> NApplyTy A1 V -> ApplyTy A2 V B2 -> B2 <: B. *)
+
+(* (* B.15 (4) *) *)
+(* Lemma applyty_orl_sub : forall (A1 A2 B B1 B2 : typ) (V:Fty), *)
+(*     ApplyTy (A1|A2) V B -> ApplyTy A1 V B1 -> ApplyTy A2 V B2 -> B <: B1 | B2. *)
+
+  (* apply(A1, Fty) => A1' *)
+  (* apply(A2, Fty) => A2' *)
+  (* ------------------------------------------ *)
+  (* apply(A1 & A2, Fty) => D /\ D <: A1'&A2' *)
+
+Lemma applyty_and_1 : forall (A1 A2 B1 B2 : typ) (V:Fty),
+    TypeWF nil (A1&A2) -> isValFty V ->
+    ApplyTy A1 V B1 -> ApplyTy A2 V B2 -> exists B, ApplyTy (A1&A2) V B /\ B1&B2 <: B.
+Proof with subst; try eassumption.
+  introv WF Val App1 App2.
+  forwards (?&Sub1&App1'): monotonicity_applyty_1 (A1&A2) App1. convert2asub. now eauto.
+  forwards (?&Sub2&App2'): monotonicity_applyty_1 (A1&A2) App2. convert2asub. now eauto.
+  forwards: applyty_unique App1' App2'...
+  forwards: applyty_andl_sub_1 App1'...
+  exists*.
+Qed.
+
+ (*****************************************************************************)
+Lemma napplytyls_sound : forall A B,
+    NApplyTyLs A B -> NApplyTy A B.
+Proof with try eassumption; new_elia.
+  introv H.
+  indTypFtySize (size_typ A + size_Fty B).
+  lets~ [?|(?&?&?&?&?)]: (ordu_or_split_Fty B). admit.
+  - inverts~ H.
+    all: forwards: IH; [eassumption | new_elia | eauto ].
+    + clear H2. forwards: IH; [eassumption | new_elia | eauto ].
+  - subst. inverts H; solve_false.
+    + clear IH SizeInd H1. induction* H0.
+    + clear IH SizeInd H1. induction* H0.
+    + clear IH SizeInd H1. induction* H0.
+    + clear IH SizeInd H1. eauto.
+    + forwards~ [?|?]: applyty_total (t_arrow A0 A') (fty_StackArg x).
+      destruct_conj.
+      forwards: applyty_soundness_1 H.
+      false. apply H5. convert2asub. auto_inv.
+    +
+Admitted.
+
+Lemma applytyls_sound : forall A B C,
+    ApplyTyLs A B C -> exists C' , ApplyTy A B C' /\ C' <: C.
+Proof with try eassumption; new_elia.
+  introv App.
+  indTypFtySize (size_typ A + size_Fty B).
+  lets~ [?|(?&?&?&?&?)]: (ordu_or_split_Fty B). admit.
+  - (* easy cases *) admit.
+    (* inverts App; solve_false. *)
+    (* 1: exists; split*. *)
+  - Local Ltac applyih IH := forwards: IH; [ | eassumption | |..].
+    inverts* App.
+    + exists. split~.
+Admitted.
+(*   - applyih IH... clear H1. *)
+(*     applyih IH... destruct_conj. *)
+(*     exists. split. eauto. admit. *)
+(*   - applyih IH... clear H1. *)
+(*     applyih IH... destruct_conj. *)
+(*     (* new_splu case *) *)
+(*     (* forwards (D1&D2&HDS) : nsplu2splu... forwards HDS' : splu2nsplu HDS. *) *)
+(*     (* exists. split. eauto. admit. *) *)
+(*     inverts H. (* 5 cases for all new_splu *) *)
+(*     + exists. split. eauto. admit. *)
+(*     + forwards (D1&D2&HDS) : nsplu2splu... *)
+(*       exists. split. applys* ApplyTyUnionArg. *)
+
+
+(* (*     intros; applys HL... now eauto. *) *)
+(*   - forwards: IH; [ | eassumption | |..]; new_elia. intros; applys HL... now eauto. *)
+(*   - forwards (D1&D2&HDS) : nsplu2splu; [eassumption | ..]; eauto. *)
+(*     forwards HDS' : splu2nsplu HDS. *)
+(*     eapply NApplyTyAltUnionArgL in H1... *)
+(*     forwards [HN|HN]: HL HDS'... *)
+(*     all: forwards*: IH HN... *)
+(*     all: intros; applys HL... *)
+(*   - forwards (D1&D2&HDS) : nsplu2splu; [eassumption | ..]; eauto. *)
+(*     forwards HDS' : splu2nsplu HDS. *)
+(*     eapply NApplyTyAltUnionArgR in H1... *)
+(*     forwards [HN|HN]: HL HDS'... *)
+(*     all: forwards*: IH HN... *)
+(*     all: intros; applys HL... *)
+(*   - forwards: IH H1... all: forwards: IH H2... *)
+(*     1-3 : intros; applys HL... *)
+(*     now eauto. *)
+(* Qed. *)
+
+Lemma typsubst_typ_applytyls : forall (A B C D : typ) X,
+  ApplyTyLs A B C -> lc_typ D ->
+  ApplyTyLs ([X ~~> D] A) ([X ~~> D] B) ([X ~~> D] C).
+Admitted. (* I removed all ordu condition in ApplyTyAlt to make this trivially true *)
+
+(* Lemma typsubst_typ_applyty : forall (A B C D : typ) X, *)
+(*   ApplyTy A B C -> lc_typ D -> *)
+(*   exists C', ApplyTy ([X ~~> D] A) ([X ~~> D] B) C' /\ C' <: ([X ~~> D] C). *)
+(* Proof. *)
+(*   introv App Lc. *)
+(*   apply applytyalt_complete in App. *)
+(*   forwards App': typsubst_typ_applytyalt X App Lc. *)
+(*   forwards (?&?&?): applytyalt_sound App'. *)
+(*   eauto. *)
+(* Qed. *)
+
+
+Lemma typsubst_applyty_ord : forall (A B C U : typ) X,
+    ApplyTy A B C -> lc_typ U -> ordu B ->
+    exists C', ApplyTy ([X ~~> U] A) ([X ~~> U] B) C' /\ C' <: [X ~~> U] C .
+Proof with try eassumption.
+  introv App Lc Ord.
+  inverts App. 4: now solve_false.
+  all: applys applytyls_sound.
+  all: applys typsubst_typ_applytyls.
+  all: eauto.
+  - (* DOES NOT HAVE ApplyTyLs premises! *)
+    (* applys ApplyTyLsUnion... *)
+  Admitted.
+
+(* At least we can prove after substitution the application must have a result (applicable): *)
+(* Consider two special substitution: *)
+(*   (1) use [X/Top] for all positive X and use [X/Bot] for all negative X *)
+(*   (2) the reverse *)
+(* A subst by (1) = a supertype of A *)
+(* A subst by (2) = a subtype of A *)
+(* Any normal substitution is between (1) and (2) *)
+(* When A is applicable to B, by monotonicity we know A(1) is applicable to B(2). *)
+(* --CANNOT PROCEED HERE-- *)
+
+Lemma typsubst_applyty : forall (A B C U : typ) X,
+    ApplyTy A B C -> lc_typ U ->
+    exists C', ApplyTy ([X ~~> U] A) ([X ~~> U] B) C' /\ C' <: [X ~~> U] C.
+Proof with try reflexivity; try eassumption.
+  introv App Lc.
+  inductions App.
+  all: try forwards: IHApp...
+  all: try forwards: IHApp1...
+  all: try forwards: IHApp2...
+  4: { destruct_conj.
+       forwards App: ApplyTyUnionArg H0 H1. applys* SpU_or.
+       forwards App': applyty_iso App.
+       now applys* iso_refl.
+       apply splu_iso in H. eapply typsubst_iso in H. simpl in H.
+       now applys~ H. now auto. destruct_conj.
+       exists. split... simpl. applys DSub_Trans H4.
+       convert2asub. match_or...
+  }
+  all : applys typsubst_applyty_ord...
+  all : try solve [inverts~ H].
+  all : try solve [inverts~ H0].
+Qed.
